

1. Consider the boundary value problem (12.1)-(12.2) with $f(x) = 1/x$. Using (12.3) prove that $u(x) = -x \log(x)$. This shows that $u \in C^2(0, 1)$ but $u(0)$ is not defined and u' , u'' do not exist at $x = 0$ (\Rightarrow : if $f \in C^0(0, 1)$, but not $f \in C^0([0, 1])$, then u does not belong to $C^0([0, 1])$).

$$(12.1): -u''(x) = f(x) = 1/x, \quad 0 < x < 1.$$

$$(12.2): u(0) = u(1) = 0.$$

$$(12.3): u(x) = \int_0^1 G(x, s) f(s) ds, \text{ where, for any fixed } x,$$
$$G(x, s) = \begin{cases} s(1-x) & \text{if } 0 \leq s \leq x, \\ x(1-s) & \text{if } x \leq s \leq 1. \end{cases}$$

$$\begin{aligned} u(x) &= \int_0^1 G(x, s) \frac{1}{s} ds \\ &= \int_0^x s(1-x) \frac{1}{s} ds + \int_x^1 x(1-s) \frac{1}{s} ds \\ &= (1-x)x + x \left[\int_x^1 \frac{1}{s} ds - \int_x^1 1 ds \right] \\ &= (1-x)x + x [\ln s|_x^1 - (1-x)] \\ &= -x \ln x \quad \text{for } 0 < x < 1. \end{aligned}$$

$$\Rightarrow u'(x) = -\ln x - 1 \Rightarrow u''(x) = -\frac{1}{x}.$$

So u' , u'' do not exist at $x=0$ and $u \in C^2(0, 1)$. \square

Cerify the summation by parts formula

$$\sum_{j=0}^{n-1} (w_{j+1} - w_j) v_j = w_n v_n - w_0 v_0 - \sum_{j=0}^{n-1} (v_{j+1} - v_j) w_{j+1},$$

and show that, for $v_h \in V_h^0$,

$$(L_h v_h, v_h)_h = h^{-1} \sum_{j=0}^{n-1} (v_{j+1} - v_j)^2.$$

(1)

$$\begin{aligned} \sum_{j=0}^{n-1} (w_{j+1} - w_j) v_j &= \sum_{j=0}^{n-1} w_{j+1} v_j - \sum_{j=0}^{n-1} w_j v_j \\ &= \sum_{j=1}^n w_j v_{j-1} - \sum_{j=0}^{n-1} w_j v_j \\ &= w_n v_{n-1} - w_0 v_0 - \sum_{j=1}^{n-1} (v_j - v_{j-1}) w_j \\ &= w_n v_{n-1} - w_0 v_0 - \sum_{j=0}^{n-2} (v_{j+1} - v_j) w_{j+1} \\ &= w_n v_{n-1} - w_0 v_0 + (v_n - v_{n-1}) w_n - \sum_{j=0}^{n-1} (v_{j+1} - v_j) w_{j+1} \\ &= w_n v_n - w_0 v_0 - \sum_{j=0}^{n-1} (v_{j+1} - v_j) w_{j+1} \end{aligned}$$

(2)

$$(L_h v_h)(x_j) = - \frac{v_h(x_{j+1}) - 2v_h(x_j) + v_h(x_{j-1}))}{h^2}, \quad j = 1 \sim n-1.$$

$(w_h, v_h)_h = h \sum_{k=0}^n c_k w_k v_k$ for two discrete functions $w_h, v_h \in V_h$, where $c_0 = c_n = 1/2$ and $c_k = 1$ for $k = 1 \sim n-1$.

Since $v_h \in V_h^0$, $v_h(x_0) = v_h(x_n) = 0$.

$$\begin{aligned} \text{So } (L_h v_h, v_h)_h &= h \sum_{j=1}^{n-1} (L_h v_h)(x_j) v_h(x_j) \\ &= h \sum_{j=1}^{n-1} \left(- \frac{v_h(x_{j+1}) - 2v_h(x_j) + v_h(x_{j-1}))}{h^2} \right) v_h(x_j) \end{aligned}$$

$$\begin{aligned} &= -\frac{1}{h} \sum_{j=1}^{n-1} [v_h(x_{j+1}) - 2v_h(x_j) + v_h(x_{j-1}))] v_h(x_j) \\ &= -\frac{1}{h} \sum_{j=1}^{n-1} [v_h(x_{j+1}) - v_h(x_j)] v_h(x_j) - [v_h(x_j) - v_h(x_{j-1}))] v_h(x_j) \\ &= -\frac{1}{h} \{ [v_h(x_2) - v_h(x_1)] v_h(x_1) - [v_h(x_1) - v_h(x_0)] v_h(x_1) \\ &\quad + [v_h(x_3) - v_h(x_2)] v_h(x_2) - [v_h(x_2) - v_h(x_1)] v_h(x_2) \\ &\quad + \dots + [v_h(x_n) - v_h(x_{n-1})] v_h(x_{n-1}) - [v_h(x_{n-1}) - v_h(x_{n-2})] v_h(x_{n-1}) \} \\ &= \frac{1}{h} \sum_{j=0}^{n-1} [v_h(x_{j+1}) - v_h(x_j)]^2 \quad \square \end{aligned}$$

Note: $v_h \in V_h^0$
 $(v_1 - v_0)^2 \uparrow = v_1^2$
 $(v_2 - v_1)^2$
 \vdots
 $(v_{n-1} - v_{n-2})^2$
 $(v_n - v_{n-1})^2 = v_{n-1}^2$

6. Prove that $G^k(x_j) = hG(x_j, x_k)$, where G is Green's function introduced in (12.4) and G^k is its corresponding discrete counterpart solution of (12.4).

[Solution: we prove the result by verifying that $L_h G = h e^k$. Indeed, for a fixed x_k the function $G(x_k, s)$ is a straight line on the intervals $[0, x_k]$ and $[x_k, 1]$ so that $L_h G = 0$ at every node x_l with $l = 0, \dots, k-1$ and $l = k+1, \dots, n+1$. Finally, a direct computation shows that $(L_h G)(x_k) = 1/h$ which concludes the proof.]

$$(12.4): G(x, s) = \begin{cases} s(1-x) & \text{if } 0 \leq s \leq x, \\ x(1-s) & \text{if } x \leq s \leq 1 \end{cases} \text{ for any fixed } x.$$

$$\text{Define } G^k(x_j) = h G(x_j, x_k).$$

① Assume $j \neq k$.

$$\text{① For } j < k, \quad G(x_j, x_k) = x_j(1-x_k).$$

$$\text{So } G(x_{j+1}, x_k) - G(x_j, x_k) = (x_{j+1} - x_j)(1-x_k) = h(1-x_k) = (x_j - x_{j+1})(1-x_k) = G(x_j, x_k) - G(x_{j+1}, x_k).$$

$$\Rightarrow G(x_{j+1}, x_k) - 2G(x_j, x_k) + G(x_{j+1}, x_k) = 0$$

$$\text{② For } j > k, \quad G(x_j, x_k) = x_k(1-x_j).$$

$$\text{So } G(x_{j+1}, x_k) - G(x_j, x_k) = x_k(x_j - x_{j+1}) = -hx_k = x_k(x_{j+1} - x_j) = G(x_j, x_k) - G(x_{j+1}, x_k).$$

$$\Rightarrow G(x_{j+1}, x_k) - 2G(x_j, x_k) + G(x_{j+1}, x_k) = 0$$

$$\text{Thus } (L_h G^k)(x_j) = \frac{G^k(x_{j+1}) - 2G^k(x_j) + G^k(x_{j-1}))}{h^2} = \frac{h[G(x_{j+1}, x_k) - 2G(x_j, x_k) + G(x_{j-1}, x_k)]}{h^2}$$

$$= 0 \text{ for } j \neq k.$$

② Assume $j = k$.

$$G(x_{k+1}, x_k) - 2G(x_k, x_k) + G(x_{k-1}, x_k)$$

$$= x_{k+1}(1-x_k) - 2x_k(1-x_k) + x_{k-1}(1-x_k)$$

$$= (k-1)h(1-kh) - 2kh(1-kh) + kh(1-(k+1)h)$$

$$= [(k-1)h - kh](1-kh) + \{- (1-kh) + [1-(k+1)h]\} kh$$

$$= -h(1-kh) - h(kh) = -h$$

$$\text{Thus } (L_h G^k)(x_j) = -\frac{h(1-h)}{h^2} = 1 \text{ for } j = k.$$

$$\text{By ①, ②, } (L_h G^k)(x_j) = \begin{cases} 0 & (j \neq k) \\ 1 & (j = k) \end{cases} = e_k.$$

$$\text{So } G^k(x_j) = h G(x_j, x_k). \quad \square$$